\begin{itemize} 
\item $(a+b) \operatorname{mod} p= (a \operatorname{mod} p +b \operatorname{mod} p ) \operatorname{mod} p$
\item $(a-b) \operatorname{mod} p= (a \operatorname{mod} p -b \operatorname{mod} p +p) \operatorname{mod} p$
\item $(a*b) \operatorname{mod} p= (a \operatorname{mod} p\cdot b \operatorname{mod} p ) \operatorname{mod} p$
\item $(a^b) \operatorname{mod} p= ((a \operatorname{mod} p )^b) \operatorname{mod} p$
\item $((a+b) \operatorname{mod} p+c) \operatorname{mod} p = (a+(b+c)) \operatorname{mod} p$
\item $((a\cdot b) \operatorname{mod} p\cdot c) \operatorname{mod} p = (a\cdot (b\cdot c)) \operatorname{mod} p$
\item $(a+b) \operatorname{mod} p=(b+a) \operatorname{mod} p$
\item $(a\cdot b) \operatorname{mod} p=(b\cdot a) \operatorname{mod} p$
\item $((a+b) \operatorname{mod} p\cdot c)= ((a\cdot c) \operatorname{mod} p +(b\cdot c) \operatorname{mod} p ) \operatorname{mod} p$

\item $a\equiv b \quad (\operatorname{mod} m) \Rightarrow c \cdot m  = a - b , c \in \mathbb{Z}\\\Rightarrow a \equiv b\quad ( \operatorname{mod} m ) \Rightarrow m \; | \; a-b$
\item $a \equiv b \quad (\operatorname{mod} c) , b \equiv d \quad (\operatorname{mod} c)\\ å‰‡\ a \equiv d (\operatorname{mod} c)$
\end{itemize}